restore flippable inv

pulse/src/ocaml/plugin/generated/Pulse_Checker_WithInv.ml
@@ -334,45 +334,123 @@ let rec (find_inv :
     Pulse_Syntax_Base.term ->
       unit ->
         Pulse_Syntax_Base.term ->
-          (Pulse_Syntax_Base.term, Pulse_Syntax_Base.term, unit, unit, 
-            unit) FStar_Pervasives.dtuple5 FStar_Pervasives_Native.option)
+          ((Pulse_Syntax_Base.term, Pulse_Syntax_Base.term, unit, unit, 
+             unit) FStar_Pervasives.dtuple5 FStar_Pervasives_Native.option,
+            unit) FStar_Tactics_Effect.tac_repr)
   =
-  fun g ->
-    fun pre ->
-      fun pre_typing ->
-        fun i ->
-          match Pulse_Syntax_Pure.inspect_term pre with
-          | Pulse_Syntax_Pure.Tm_Inv (i', p) ->
-              if Pulse_Syntax_Base.eq_tm i i'
-              then
-                let frame = Pulse_Syntax_Pure.tm_emp in
-                FStar_Pervasives_Native.Some
-                  (FStar_Pervasives.Mkdtuple5 (p, frame, (), (), ()))
-              else FStar_Pervasives_Native.None
-          | Pulse_Syntax_Pure.Tm_Star (l, r) ->
-              (match find_inv g l () i with
-               | FStar_Pervasives_Native.Some res ->
-                   let uu___ = res in
-                   (match uu___ with
-                    | FStar_Pervasives.Mkdtuple5
-                        (p, frame, uu___1, uu___2, uu___3) ->
-                        FStar_Pervasives_Native.Some
-                          (FStar_Pervasives.Mkdtuple5
-                             (p, (Pulse_Syntax_Pure.tm_star frame r), (), (),
-                               ())))
-               | FStar_Pervasives_Native.None ->
-                   (match find_inv g r () i with
-                    | FStar_Pervasives_Native.Some res ->
-                        let uu___ = res in
-                        (match uu___ with
-                         | FStar_Pervasives.Mkdtuple5
-                             (p, frame, uu___1, uu___2, uu___3) ->
-                             FStar_Pervasives_Native.Some
-                               (FStar_Pervasives.Mkdtuple5
-                                  (p, (Pulse_Syntax_Pure.tm_star l frame),
-                                    (), (), ())))
-                    | uu___ -> FStar_Pervasives_Native.None))
-          | uu___ -> FStar_Pervasives_Native.None
+  fun uu___3 ->
+    fun uu___2 ->
+      fun uu___1 ->
+        fun uu___ ->
+          (fun g ->
+             fun pre ->
+               fun pre_typing ->
+                 fun i ->
+                   match Pulse_Syntax_Pure.inspect_term pre with
+                   | Pulse_Syntax_Pure.Tm_Inv (i', p) ->
+                       Obj.magic
+                         (Obj.repr
+                            (FStar_Tactics_Effect.lift_div_tac
+                               (fun uu___ ->
+                                  if Pulse_Syntax_Base.eq_tm i i'
+                                  then
+                                    FStar_Pervasives_Native.Some
+                                      (FStar_Pervasives.Mkdtuple5
+                                         (p, Pulse_Syntax_Pure.tm_emp, (),
+                                           (), ()))
+                                  else FStar_Pervasives_Native.None)))
+                   | Pulse_Syntax_Pure.Tm_Star (l, r) ->
+                       Obj.magic
+                         (Obj.repr
+                            (FStar_Tactics_Effect.tac_bind
+                               (FStar_Sealed.seal
+                                  (Obj.magic
+                                     (FStar_Range.mk_range
+                                        "Pulse.Checker.WithInv.fst"
+                                        (Prims.of_int (195))
+                                        (Prims.of_int (10))
+                                        (Prims.of_int (195))
+                                        (Prims.of_int (37)))))
+                               (FStar_Sealed.seal
+                                  (Obj.magic
+                                     (FStar_Range.mk_range
+                                        "Pulse.Checker.WithInv.fst"
+                                        (Prims.of_int (195))
+                                        (Prims.of_int (4))
+                                        (Prims.of_int (204))
+                                        (Prims.of_int (17)))))
+                               (Obj.magic (find_inv g l () i))
+                               (fun uu___ ->
+                                  (fun uu___ ->
+                                     match uu___ with
+                                     | FStar_Pervasives_Native.Some res ->
+                                         Obj.magic
+                                           (Obj.repr
+                                              (FStar_Tactics_Effect.lift_div_tac
+                                                 (fun uu___1 ->
+                                                    match res with
+                                                    | FStar_Pervasives.Mkdtuple5
+                                                        (p, frame, uu___2,
+                                                         uu___3, uu___4)
+                                                        ->
+                                                        FStar_Pervasives_Native.Some
+                                                          (FStar_Pervasives.Mkdtuple5
+                                                             (p,
+                                                               (Pulse_Syntax_Pure.tm_star
+                                                                  frame r),
+                                                               (), (), ())))))
+                                     | FStar_Pervasives_Native.None ->
+                                         Obj.magic
+                                           (Obj.repr
+                                              (FStar_Tactics_Effect.tac_bind
+                                                 (FStar_Sealed.seal
+                                                    (Obj.magic
+                                                       (FStar_Range.mk_range
+                                                          "Pulse.Checker.WithInv.fst"
+                                                          (Prims.of_int (200))
+                                                          (Prims.of_int (12))
+                                                          (Prims.of_int (200))
+                                                          (Prims.of_int (39)))))
+                                                 (FStar_Sealed.seal
+                                                    (Obj.magic
+                                                       (FStar_Range.mk_range
+                                                          "Pulse.Checker.WithInv.fst"
+                                                          (Prims.of_int (200))
+                                                          (Prims.of_int (6))
+                                                          (Prims.of_int (204))
+                                                          (Prims.of_int (17)))))
+                                                 (Obj.magic
+                                                    (find_inv g r () i))
+                                                 (fun uu___1 ->
+                                                    FStar_Tactics_Effect.lift_div_tac
+                                                      (fun uu___2 ->
+                                                         match uu___1 with
+                                                         | FStar_Pervasives_Native.Some
+                                                             res ->
+                                                             (match res with
+                                                              | FStar_Pervasives.Mkdtuple5
+                                                                  (p, frame,
+                                                                   uu___3,
+                                                                   uu___4,
+                                                                   uu___5)
+                                                                  ->
+                                                                  FStar_Pervasives_Native.Some
+                                                                    (
+                                                                    FStar_Pervasives.Mkdtuple5
+                                                                    (p,
+                                                                    (Pulse_Syntax_Pure.tm_star
+                                                                    l frame),
+                                                                    (), (),
+                                                                    ())))
+                                                         | uu___3 ->
+                                                             FStar_Pervasives_Native.None)))))
+                                    uu___)))
+                   | uu___ ->
+                       Obj.magic
+                         (Obj.repr
+                            (FStar_Tactics_Effect.lift_div_tac
+                               (fun uu___1 -> FStar_Pervasives_Native.None))))
+            uu___3 uu___2 uu___1 uu___
 let (find_inv_post :
   Pulse_Typing_Env.env ->
     Pulse_Syntax_Base.var ->
@@ -430,12 +508,11 @@ let (find_inv_post :
                                         (Prims.of_int (2))
                                         (Prims.of_int (233))
                                         (Prims.of_int (71)))))
-                               (FStar_Tactics_Effect.lift_div_tac
-                                  (fun uu___ ->
-                                     find_inv
-                                       (Pulse_Typing_Env.push_binding g x
-                                          Pulse_Syntax_Base.ppname_default
-                                          ret_ty) post_opened () i))
+                               (Obj.magic
+                                  (find_inv
+                                     (Pulse_Typing_Env.push_binding g x
+                                        Pulse_Syntax_Base.ppname_default
+                                        ret_ty) post_opened () i))
                                (fun uu___ ->
                                   (fun res ->
                                      match res with
@@ -569,7 +646,7 @@ let (check :
                      (Obj.magic
                         (FStar_Range.mk_range "Pulse.Checker.WithInv.fst"
                            (Prims.of_int (287)) Prims.int_one
-                           (Prims.of_int (469)) (Prims.of_int (59)))))
+                           (Prims.of_int (473)) (Prims.of_int (59)))))
                   (FStar_Tactics_Effect.lift_div_tac
                      (fun uu___ -> t.Pulse_Syntax_Base.term1))
                   (fun uu___ ->
@@ -586,145 +663,186 @@ let (check :
                                     (Obj.magic
                                        (FStar_Range.mk_range
                                           "Pulse.Checker.WithInv.fst"
-                                          (Prims.of_int (289))
-                                          (Prims.of_int (4))
-                                          (Prims.of_int (300))
-                                          (Prims.of_int (67)))))
+                                          (Prims.of_int (288))
+                                          (Prims.of_int (19))
+                                          (Prims.of_int (288))
+                                          (Prims.of_int (50)))))
                                  (FStar_Sealed.seal
                                     (Obj.magic
                                        (FStar_Range.mk_range
                                           "Pulse.Checker.WithInv.fst"
-                                          (Prims.of_int (308))
-                                          (Prims.of_int (8))
-                                          (Prims.of_int (469))
+                                          (Prims.of_int (287))
+                                          (Prims.of_int (56))
+                                          (Prims.of_int (473))
                                           (Prims.of_int (59)))))
-                                 (match (returns_inv, post_hint) with
-                                  | (FStar_Pervasives_Native.None,
-                                     FStar_Pervasives_Native.Some p) ->
-                                      Obj.magic
-                                        (Obj.repr
-                                           (FStar_Tactics_Effect.lift_div_tac
-                                              (fun uu___1 -> p)))
-                                  | (FStar_Pervasives_Native.Some (b, p),
-                                     FStar_Pervasives_Native.None) ->
-                                      Obj.magic
-                                        (Obj.repr
-                                           (Pulse_Checker_Base.intro_post_hint
-                                              g
-                                              Pulse_Syntax_Base.EffectAnnotSTT
-                                              (FStar_Pervasives_Native.Some
-                                                 (b.Pulse_Syntax_Base.binder_ty))
-                                              p))
-                                  | (FStar_Pervasives_Native.Some
-                                     (uu___1, p),
-                                     FStar_Pervasives_Native.Some q) ->
-                                      Obj.magic
-                                        (Obj.repr
-                                           (FStar_Tactics_Effect.tac_bind
-                                              (FStar_Sealed.seal
-                                                 (Obj.magic
-                                                    (FStar_Range.mk_range
-                                                       "Pulse.Checker.WithInv.fst"
-                                                       (Prims.of_int (296))
-                                                       (Prims.of_int (8))
-                                                       (Prims.of_int (298))
-                                                       (Prims.of_int (60)))))
-                                              (FStar_Sealed.seal
-                                                 (Obj.magic
-                                                    (FStar_Range.mk_range
-                                                       "Pulse.Checker.WithInv.fst"
-                                                       (Prims.of_int (295))
-                                                       (Prims.of_int (6))
-                                                       (Prims.of_int (298))
-                                                       (Prims.of_int (60)))))
-                                              (Obj.magic
-                                                 (FStar_Tactics_Effect.tac_bind
-                                                    (FStar_Sealed.seal
-                                                       (Obj.magic
-                                                          (FStar_Range.mk_range
-                                                             "Pulse.Checker.WithInv.fst"
-                                                             (Prims.of_int (296))
-                                                             (Prims.of_int (8))
-                                                             (Prims.of_int (298))
-                                                             (Prims.of_int (60)))))
-                                                    (FStar_Sealed.seal
-                                                       (Obj.magic
-                                                          (FStar_Range.mk_range
-                                                             "Pulse.Checker.WithInv.fst"
-                                                             (Prims.of_int (296))
-                                                             (Prims.of_int (8))
-                                                             (Prims.of_int (298))
-                                                             (Prims.of_int (60)))))
-                                                    (Obj.magic
-                                                       (FStar_Tactics_Effect.tac_bind
-                                                          (FStar_Sealed.seal
-                                                             (Obj.magic
-                                                                (FStar_Range.mk_range
-                                                                   "Pulse.Checker.WithInv.fst"
-                                                                   (Prims.of_int (297))
-                                                                   (Prims.of_int (10))
-                                                                   (Prims.of_int (297))
-                                                                   (Prims.of_int (57)))))
-                                                          (FStar_Sealed.seal
-                                                             (Obj.magic
-                                                                (FStar_Range.mk_range
-                                                                   "Pulse.Checker.WithInv.fst"
-                                                                   (Prims.of_int (296))
-                                                                   (Prims.of_int (8))
-                                                                   (Prims.of_int (298))
-                                                                   (Prims.of_int (60)))))
-                                                          (Obj.magic
-                                                             (FStar_Tactics_Effect.tac_bind
-                                                                (FStar_Sealed.seal
-                                                                   (Obj.magic
-                                                                    (FStar_Range.mk_range
-                                                                    "Pulse.Checker.WithInv.fst"
-                                                                    (Prims.of_int (297))
-                                                                    (Prims.of_int (51))
-                                                                    (Prims.of_int (297))
-                                                                    (Prims.of_int (57)))))
-                                                                (FStar_Sealed.seal
-                                                                   (Obj.magic
-                                                                    (FStar_Range.mk_range
-                                                                    "Pulse.Checker.WithInv.fst"
-                                                                    (Prims.of_int (297))
-                                                                    (Prims.of_int (10))
-                                                                    (Prims.of_int (297))
-                                                                    (Prims.of_int (57)))))
+                                 (Obj.magic
+                                    (Pulse_Checker_Pure.check_tot_term g i
+                                       Pulse_Syntax_Pure.tm_iname_ref))
+                                 (fun uu___1 ->
+                                    (fun uu___1 ->
+                                       match uu___1 with
+                                       | Prims.Mkdtuple2 (i1, uu___2) ->
+                                           Obj.magic
+                                             (FStar_Tactics_Effect.tac_bind
+                                                (FStar_Sealed.seal
+                                                   (Obj.magic
+                                                      (FStar_Range.mk_range
+                                                         "Pulse.Checker.WithInv.fst"
+                                                         (Prims.of_int (291))
+                                                         (Prims.of_int (4))
+                                                         (Prims.of_int (302))
+                                                         (Prims.of_int (67)))))
+                                                (FStar_Sealed.seal
+                                                   (Obj.magic
+                                                      (FStar_Range.mk_range
+                                                         "Pulse.Checker.WithInv.fst"
+                                                         (Prims.of_int (310))
+                                                         (Prims.of_int (8))
+                                                         (Prims.of_int (473))
+                                                         (Prims.of_int (59)))))
+                                                (match (returns_inv,
+                                                         post_hint)
+                                                 with
+                                                 | (FStar_Pervasives_Native.None,
+                                                    FStar_Pervasives_Native.Some
+                                                    p) ->
+                                                     Obj.magic
+                                                       (Obj.repr
+                                                          (FStar_Tactics_Effect.lift_div_tac
+                                                             (fun uu___3 -> p)))
+                                                 | (FStar_Pervasives_Native.Some
+                                                    (b, p),
+                                                    FStar_Pervasives_Native.None)
+                                                     ->
+                                                     Obj.magic
+                                                       (Obj.repr
+                                                          (Pulse_Checker_Base.intro_post_hint
+                                                             g
+                                                             (Pulse_Syntax_Base.EffectAnnotAtomic
+                                                                {
+                                                                  Pulse_Syntax_Base.opens1
+                                                                    =
+                                                                    (
+                                                                    Pulse_Reflection_Util.add_inv_tm
+                                                                    Pulse_Syntax_Pure.tm_emp_inames
+                                                                    i1)
+                                                                })
+                                                             (FStar_Pervasives_Native.Some
+                                                                (b.Pulse_Syntax_Base.binder_ty))
+                                                             p))
+                                                 | (FStar_Pervasives_Native.Some
+                                                    (uu___3, p),
+                                                    FStar_Pervasives_Native.Some
+                                                    q) ->
+                                                     Obj.magic
+                                                       (Obj.repr
+                                                          (FStar_Tactics_Effect.tac_bind
+                                                             (FStar_Sealed.seal
                                                                 (Obj.magic
-                                                                   (Pulse_PP.pp
+                                                                   (FStar_Range.mk_range
+                                                                    "Pulse.Checker.WithInv.fst"
+                                                                    (Prims.of_int (298))
+                                                                    (Prims.of_int (8))
+                                                                    (Prims.of_int (300))
+                                                                    (Prims.of_int (60)))))
+                                                             (FStar_Sealed.seal
+                                                                (Obj.magic
+                                                                   (FStar_Range.mk_range
+                                                                    "Pulse.Checker.WithInv.fst"
+                                                                    (Prims.of_int (297))
+                                                                    (Prims.of_int (6))
+                                                                    (Prims.of_int (300))
+                                                                    (Prims.of_int (60)))))
+                                                             (Obj.magic
+                                                                (FStar_Tactics_Effect.tac_bind
+                                                                   (FStar_Sealed.seal
+                                                                    (Obj.magic
+                                                                    (FStar_Range.mk_range
+                                                                    "Pulse.Checker.WithInv.fst"
+                                                                    (Prims.of_int (298))
+                                                                    (Prims.of_int (8))
+                                                                    (Prims.of_int (300))
+                                                                    (Prims.of_int (60)))))
+                                                                   (FStar_Sealed.seal
+                                                                    (Obj.magic
+                                                                    (FStar_Range.mk_range
+                                                                    "Pulse.Checker.WithInv.fst"
+                                                                    (Prims.of_int (298))
+                                                                    (Prims.of_int (8))
+                                                                    (Prims.of_int (300))
+                                                                    (Prims.of_int (60)))))
+                                                                   (Obj.magic
+                                                                    (FStar_Tactics_Effect.tac_bind
+                                                                    (FStar_Sealed.seal
+                                                                    (Obj.magic
+                                                                    (FStar_Range.mk_range
+                                                                    "Pulse.Checker.WithInv.fst"
+                                                                    (Prims.of_int (299))
+                                                                    (Prims.of_int (10))
+                                                                    (Prims.of_int (299))
+                                                                    (Prims.of_int (57)))))
+                                                                    (FStar_Sealed.seal
+                                                                    (Obj.magic
+                                                                    (FStar_Range.mk_range
+                                                                    "Pulse.Checker.WithInv.fst"
+                                                                    (Prims.of_int (298))
+                                                                    (Prims.of_int (8))
+                                                                    (Prims.of_int (300))
+                                                                    (Prims.of_int (60)))))
+                                                                    (Obj.magic
+                                                                    (FStar_Tactics_Effect.tac_bind
+                                                                    (FStar_Sealed.seal
+                                                                    (Obj.magic
+                                                                    (FStar_Range.mk_range
+                                                                    "Pulse.Checker.WithInv.fst"
+                                                                    (Prims.of_int (299))
+                                                                    (Prims.of_int (51))
+                                                                    (Prims.of_int (299))
+                                                                    (Prims.of_int (57)))))
+                                                                    (FStar_Sealed.seal
+                                                                    (Obj.magic
+                                                                    (FStar_Range.mk_range
+                                                                    "Pulse.Checker.WithInv.fst"
+                                                                    (Prims.of_int (299))
+                                                                    (Prims.of_int (10))
+                                                                    (Prims.of_int (299))
+                                                                    (Prims.of_int (57)))))
+                                                                    (Obj.magic
+                                                                    (Pulse_PP.pp
                                                                     Pulse_PP.printable_fstar_term
                                                                     p))
-                                                                (fun uu___2
-                                                                   ->
-                                                                   FStar_Tactics_Effect.lift_div_tac
                                                                     (fun
-                                                                    uu___3 ->
+                                                                    uu___4 ->
+                                                                    FStar_Tactics_Effect.lift_div_tac
+                                                                    (fun
+                                                                    uu___5 ->
                                                                     FStar_Pprint.prefix
                                                                     (Prims.of_int (4))
                                                                     Prims.int_one
                                                                     (Pulse_PP.text
                                                                     "First postcondition:")
-                                                                    uu___2))))
-                                                          (fun uu___2 ->
-                                                             (fun uu___2 ->
-                                                                Obj.magic
-                                                                  (FStar_Tactics_Effect.tac_bind
+                                                                    uu___4))))
+                                                                    (fun
+                                                                    uu___4 ->
+                                                                    (fun
+                                                                    uu___4 ->
+                                                                    Obj.magic
+                                                                    (FStar_Tactics_Effect.tac_bind
                                                                     (FStar_Sealed.seal
                                                                     (Obj.magic
                                                                     (FStar_Range.mk_range
                                                                     "Pulse.Checker.WithInv.fst"
-                                                                    (Prims.of_int (296))
-                                                                    (Prims.of_int (8))
                                                                     (Prims.of_int (298))
+                                                                    (Prims.of_int (8))
+                                                                    (Prims.of_int (300))
                                                                     (Prims.of_int (60)))))
                                                                     (FStar_Sealed.seal
                                                                     (Obj.magic
                                                                     (FStar_Range.mk_range
                                                                     "Pulse.Checker.WithInv.fst"
-                                                                    (Prims.of_int (296))
-                                                                    (Prims.of_int (8))
                                                                     (Prims.of_int (298))
+                                                                    (Prims.of_int (8))
+                                                                    (Prims.of_int (300))
                                                                     (Prims.of_int (60)))))
                                                                     (Obj.magic
                                                                     (FStar_Tactics_Effect.tac_bind
@@ -732,17 +850,17 @@ let (check :
                                                                     (Obj.magic
                                                                     (FStar_Range.mk_range
                                                                     "Pulse.Checker.WithInv.fst"
-                                                                    (Prims.of_int (298))
+                                                                    (Prims.of_int (300))
                                                                     (Prims.of_int (10))
-                                                                    (Prims.of_int (298))
+                                                                    (Prims.of_int (300))
                                                                     (Prims.of_int (58)))))
                                                                     (FStar_Sealed.seal
                                                                     (Obj.magic
                                                                     (FStar_Range.mk_range
                                                                     "Pulse.Checker.WithInv.fst"
-                                                                    (Prims.of_int (296))
-                                                                    (Prims.of_int (8))
                                                                     (Prims.of_int (298))
+                                                                    (Prims.of_int (8))
+                                                                    (Prims.of_int (300))
                                                                     (Prims.of_int (60)))))
                                                                     (Obj.magic
                                                                     (FStar_Tactics_Effect.tac_bind
@@ -750,143 +868,184 @@ let (check :
                                                                     (Obj.magic
                                                                     (FStar_Range.mk_range
                                                                     "Pulse.Checker.WithInv.fst"
-                                                                    (Prims.of_int (298))
+                                                                    (Prims.of_int (300))
                                                                     (Prims.of_int (52))
-                                                                    (Prims.of_int (298))
+                                                                    (Prims.of_int (300))
                                                                     (Prims.of_int (58)))))
                                                                     (FStar_Sealed.seal
                                                                     (Obj.magic
                                                                     (FStar_Range.mk_range
                                                                     "Pulse.Checker.WithInv.fst"
-                                                                    (Prims.of_int (298))
+                                                                    (Prims.of_int (300))
                                                                     (Prims.of_int (10))
-                                                                    (Prims.of_int (298))
+                                                                    (Prims.of_int (300))
                                                                     (Prims.of_int (58)))))
                                                                     (Obj.magic
                                                                     (Pulse_PP.pp
                                                                     Pulse_PP.printable_post_hint_t
                                                                     q))
                                                                     (fun
-                                                                    uu___3 ->
+                                                                    uu___5 ->
                                                                     FStar_Tactics_Effect.lift_div_tac
                                                                     (fun
-                                                                    uu___4 ->
+                                                                    uu___6 ->
                                                                     FStar_Pprint.prefix
                                                                     (Prims.of_int (4))
                                                                     Prims.int_one
                                                                     (Pulse_PP.text
                                                                     "Second postcondition:")
-                                                                    uu___3))))
+                                                                    uu___5))))
                                                                     (fun
-                                                                    uu___3 ->
+                                                                    uu___5 ->
                                                                     FStar_Tactics_Effect.lift_div_tac
                                                                     (fun
-                                                                    uu___4 ->
-                                                                    [uu___3]))))
+                                                                    uu___6 ->
+                                                                    [uu___5]))))
                                                                     (fun
-                                                                    uu___3 ->
+                                                                    uu___5 ->
                                                                     FStar_Tactics_Effect.lift_div_tac
                                                                     (fun
+                                                                    uu___6 ->
+                                                                    uu___4 ::
+                                                                    uu___5))))
+                                                                    uu___4)))
+                                                                   (fun
                                                                     uu___4 ->
-                                                                    uu___2 ::
-                                                                    uu___3))))
-                                                               uu___2)))
-                                                    (fun uu___2 ->
-                                                       FStar_Tactics_Effect.lift_div_tac
-                                                         (fun uu___3 ->
-                                                            (FStar_Pprint.doc_of_string
-                                                               "Fatal: multiple annotated postconditions on with_invariant")
-                                                            :: uu___2))))
-                                              (fun uu___2 ->
-                                                 (fun uu___2 ->
-                                                    Obj.magic
-                                                      (Pulse_Typing_Env.fail_doc
-                                                         g
-                                                         (FStar_Pervasives_Native.Some
-                                                            (t.Pulse_Syntax_Base.range1))
-                                                         uu___2)) uu___2)))
-                                  | (uu___1, uu___2) ->
-                                      Obj.magic
-                                        (Obj.repr
-                                           (Pulse_Typing_Env.fail g
-                                              (FStar_Pervasives_Native.Some
-                                                 (t.Pulse_Syntax_Base.range1))
-                                              "Fatal: no post hint on with_invariant")))
-                                 (fun uu___1 ->
-                                    (fun post_hint1 ->
-                                       Obj.magic
-                                         (FStar_Tactics_Effect.tac_bind
-                                            (FStar_Sealed.seal
-                                               (Obj.magic
-                                                  (FStar_Range.mk_range
-                                                     "Pulse.Checker.WithInv.fst"
-                                                     (Prims.of_int (311))
-                                                     (Prims.of_int (21))
-                                                     (Prims.of_int (311))
-                                                     (Prims.of_int (31)))))
-                                            (FStar_Sealed.seal
-                                               (Obj.magic
-                                                  (FStar_Range.mk_range
-                                                     "Pulse.Checker.WithInv.fst"
-                                                     (Prims.of_int (311))
-                                                     (Prims.of_int (34))
-                                                     (Prims.of_int (469))
-                                                     (Prims.of_int (59)))))
-                                            (FStar_Tactics_Effect.lift_div_tac
-                                               (fun uu___1 ->
-                                                  body.Pulse_Syntax_Base.range1))
-                                            (fun uu___1 ->
-                                               (fun body_range ->
-                                                  Obj.magic
-                                                    (FStar_Tactics_Effect.tac_bind
-                                                       (FStar_Sealed.seal
-                                                          (Obj.magic
-                                                             (FStar_Range.mk_range
-                                                                "Pulse.Checker.WithInv.fst"
-                                                                (Prims.of_int (312))
-                                                                (Prims.of_int (18))
-                                                                (Prims.of_int (312))
-                                                                (Prims.of_int (52)))))
-                                                       (FStar_Sealed.seal
-                                                          (Obj.magic
-                                                             (FStar_Range.mk_range
-                                                                "Pulse.Checker.WithInv.fst"
-                                                                (Prims.of_int (312))
-                                                                (Prims.of_int (55))
-                                                                (Prims.of_int (469))
-                                                                (Prims.of_int (59)))))
-                                                       (FStar_Tactics_Effect.lift_div_tac
-                                                          (fun uu___1 ->
-                                                             Pulse_RuntimeUtils.range_of_term
-                                                               i))
-                                                       (fun uu___1 ->
-                                                          (fun i_range ->
-                                                             Obj.magic
-                                                               (FStar_Tactics_Effect.tac_bind
-                                                                  (FStar_Sealed.seal
-                                                                    (Obj.magic
-                                                                    (FStar_Range.mk_range
+                                                                    FStar_Tactics_Effect.lift_div_tac
+                                                                    (fun
+                                                                    uu___5 ->
+                                                                    (FStar_Pprint.doc_of_string
+                                                                    "Fatal: multiple annotated postconditions on with_invariant")
+                                                                    :: uu___4))))
+                                                             (fun uu___4 ->
+                                                                (fun uu___4
+                                                                   ->
+                                                                   Obj.magic
+                                                                    (Pulse_Typing_Env.fail_doc
+                                                                    g
+                                                                    (FStar_Pervasives_Native.Some
+                                                                    (t.Pulse_Syntax_Base.range1))
+                                                                    uu___4))
+                                                                  uu___4)))
+                                                 | (uu___3, uu___4) ->
+                                                     Obj.magic
+                                                       (Obj.repr
+                                                          (Pulse_Typing_Env.fail
+                                                             g
+                                                             (FStar_Pervasives_Native.Some
+                                                                (t.Pulse_Syntax_Base.range1))
+                                                             "Fatal: no post hint on with_invariant")))
+                                                (fun uu___3 ->
+                                                   (fun post_hint1 ->
+                                                      Obj.magic
+                                                        (FStar_Tactics_Effect.tac_bind
+                                                           (FStar_Sealed.seal
+                                                              (Obj.magic
+                                                                 (FStar_Range.mk_range
                                                                     "Pulse.Checker.WithInv.fst"
-                                                                    (Prims.of_int (314))
-                                                                    (Prims.of_int (14))
-                                                                    (Prims.of_int (314))
-                                                                    (Prims.of_int (35)))))
-                                                                  (FStar_Sealed.seal
-                                                                    (Obj.magic
-                                                                    (FStar_Range.mk_range
+                                                                    (Prims.of_int (313))
+                                                                    (Prims.of_int (21))
+                                                                    (Prims.of_int (313))
+                                                                    (Prims.of_int (31)))))
+                                                           (FStar_Sealed.seal
+                                                              (Obj.magic
+                                                                 (FStar_Range.mk_range
                                                                     "Pulse.Checker.WithInv.fst"
-                                                                    (Prims.of_int (315))
-                                                                    (Prims.of_int (4))
-                                                                    (Prims.of_int (469))
+                                                                    (Prims.of_int (313))
+                                                                    (Prims.of_int (34))
+                                                                    (Prims.of_int (473))
                                                                     (Prims.of_int (59)))))
-                                                                  (FStar_Tactics_Effect.lift_div_tac
+                                                           (FStar_Tactics_Effect.lift_div_tac
+                                                              (fun uu___3 ->
+                                                                 body.Pulse_Syntax_Base.range1))
+                                                           (fun uu___3 ->
+                                                              (fun body_range
+                                                                 ->
+                                                                 Obj.magic
+                                                                   (FStar_Tactics_Effect.tac_bind
+                                                                    (FStar_Sealed.seal
+                                                                    (Obj.magic
+                                                                    (FStar_Range.mk_range
+                                                                    "Pulse.Checker.WithInv.fst"
+                                                                    (Prims.of_int (314))
+                                                                    (Prims.of_int (18))
+                                                                    (Prims.of_int (314))
+                                                                    (Prims.of_int (52)))))
+                                                                    (FStar_Sealed.seal
+                                                                    (Obj.magic
+                                                                    (FStar_Range.mk_range
+                                                                    "Pulse.Checker.WithInv.fst"
+                                                                    (Prims.of_int (314))
+                                                                    (Prims.of_int (55))
+                                                                    (Prims.of_int (473))
+                                                                    (Prims.of_int (59)))))
+                                                                    (FStar_Tactics_Effect.lift_div_tac
                                                                     (fun
-                                                                    uu___1 ->
-                                                                    find_inv
-                                                                    g pre ()
-                                                                    i))
-                                                                  (fun uu___1
+                                                                    uu___3 ->
+                                                                    Pulse_RuntimeUtils.range_of_term
+                                                                    i1))
+                                                                    (fun
+                                                                    uu___3 ->
+                                                                    (fun
+                                                                    i_range
                                                                     ->
+                                                                    Obj.magic
+                                                                    (FStar_Tactics_Effect.tac_bind
+                                                                    (FStar_Sealed.seal
+                                                                    (Obj.magic
+                                                                    (FStar_Range.mk_range
+                                                                    "Pulse.Checker.WithInv.fst"
+                                                                    (Prims.of_int (316))
+                                                                    (Prims.of_int (21))
+                                                                    (Prims.of_int (316))
+                                                                    (Prims.of_int (52)))))
+                                                                    (FStar_Sealed.seal
+                                                                    (Obj.magic
+                                                                    (FStar_Range.mk_range
+                                                                    "Pulse.Checker.WithInv.fst"
+                                                                    (Prims.of_int (314))
+                                                                    (Prims.of_int (55))
+                                                                    (Prims.of_int (473))
+                                                                    (Prims.of_int (59)))))
+                                                                    (Obj.magic
+                                                                    (Pulse_Checker_Pure.check_tot_term
+                                                                    g i1
+                                                                    Pulse_Syntax_Pure.tm_iname_ref))
+                                                                    (fun
+                                                                    uu___3 ->
+                                                                    (fun
+                                                                    uu___3 ->
+                                                                    match uu___3
+                                                                    with
+                                                                    | 
+                                                                    Prims.Mkdtuple2
+                                                                    (i2,
+                                                                    uu___4)
+                                                                    ->
+                                                                    Obj.magic
+                                                                    (FStar_Tactics_Effect.tac_bind
+                                                                    (FStar_Sealed.seal
+                                                                    (Obj.magic
+                                                                    (FStar_Range.mk_range
+                                                                    "Pulse.Checker.WithInv.fst"
+                                                                    (Prims.of_int (318))
+                                                                    (Prims.of_int (14))
+                                                                    (Prims.of_int (318))
+                                                                    (Prims.of_int (35)))))
+                                                                    (FStar_Sealed.seal
+                                                                    (Obj.magic
+                                                                    (FStar_Range.mk_range
+                                                                    "Pulse.Checker.WithInv.fst"
+                                                                    (Prims.of_int (319))
+                                                                    (Prims.of_int (4))
+                                                                    (Prims.of_int (473))
+                                                                    (Prims.of_int (59)))))
+                                                                    (Obj.magic
+                                                                    (find_inv
+                                                                    g pre ()
+                                                                    i2))
+                                                                    (fun
+                                                                    uu___5 ->
                                                                     (fun res
                                                                     ->
                                                                     Obj.magic
@@ -895,17 +1054,17 @@ let (check :
                                                                     (Obj.magic
                                                                     (FStar_Range.mk_range
                                                                     "Pulse.Checker.WithInv.fst"
-                                                                    (Prims.of_int (315))
+                                                                    (Prims.of_int (319))
                                                                     (Prims.of_int (4))
-                                                                    (Prims.of_int (315))
+                                                                    (Prims.of_int (319))
                                                                     (Prims.of_int (76)))))
                                                                     (FStar_Sealed.seal
                                                                     (Obj.magic
                                                                     (FStar_Range.mk_range
                                                                     "Pulse.Checker.WithInv.fst"
-                                                                    (Prims.of_int (315))
+                                                                    (Prims.of_int (319))
                                                                     (Prims.of_int (77))
-                                                                    (Prims.of_int (469))
+                                                                    (Prims.of_int (473))
                                                                     (Prims.of_int (59)))))
                                                                     (if
                                                                     FStar_Pervasives_Native.uu___is_None
@@ -923,39 +1082,39 @@ let (check :
                                                                     (Obj.repr
                                                                     (FStar_Tactics_Effect.lift_div_tac
                                                                     (fun
-                                                                    uu___2 ->
+                                                                    uu___6 ->
                                                                     ()))))
                                                                     (fun
-                                                                    uu___1 ->
+                                                                    uu___5 ->
                                                                     (fun
-                                                                    uu___1 ->
+                                                                    uu___5 ->
                                                                     Obj.magic
                                                                     (FStar_Tactics_Effect.tac_bind
                                                                     (FStar_Sealed.seal
                                                                     (Obj.magic
                                                                     (FStar_Range.mk_range
                                                                     "Pulse.Checker.WithInv.fst"
-                                                                    (Prims.of_int (317))
+                                                                    (Prims.of_int (321))
                                                                     (Prims.of_int (80))
-                                                                    (Prims.of_int (317))
+                                                                    (Prims.of_int (321))
                                                                     (Prims.of_int (83)))))
                                                                     (FStar_Sealed.seal
                                                                     (Obj.magic
                                                                     (FStar_Range.mk_range
                                                                     "Pulse.Checker.WithInv.fst"
-                                                                    (Prims.of_int (315))
+                                                                    (Prims.of_int (319))
                                                                     (Prims.of_int (77))
-                                                                    (Prims.of_int (469))
+                                                                    (Prims.of_int (473))
                                                                     (Prims.of_int (59)))))
                                                                     (FStar_Tactics_Effect.lift_div_tac
                                                                     (fun
-                                                                    uu___2 ->
+                                                                    uu___6 ->
                                                                     res))
                                                                     (fun
-                                                                    uu___2 ->
+                                                                    uu___6 ->
                                                                     (fun
-                                                                    uu___2 ->
-                                                                    match uu___2
+                                                                    uu___6 ->
+                                                                    match uu___6
                                                                     with
                                                                     | 
                                                                     FStar_Pervasives_Native.Some
@@ -972,26 +1131,26 @@ let (check :
                                                                     (Obj.magic
                                                                     (FStar_Range.mk_range
                                                                     "Pulse.Checker.WithInv.fst"
-                                                                    (Prims.of_int (319))
+                                                                    (Prims.of_int (323))
                                                                     (Prims.of_int (27))
-                                                                    (Prims.of_int (319))
+                                                                    (Prims.of_int (323))
                                                                     (Prims.of_int (46)))))
                                                                     (FStar_Sealed.seal
                                                                     (Obj.magic
                                                                     (FStar_Range.mk_range
                                                                     "Pulse.Checker.WithInv.fst"
-                                                                    (Prims.of_int (319))
+                                                                    (Prims.of_int (323))
                                                                     (Prims.of_int (49))
-                                                                    (Prims.of_int (469))
+                                                                    (Prims.of_int (473))
                                                                     (Prims.of_int (59)))))
                                                                     (FStar_Tactics_Effect.lift_div_tac
                                                                     (fun
-                                                                    uu___3 ->
+                                                                    uu___7 ->
                                                                     Pulse_Syntax_Pure.tm_star
                                                                     p
                                                                     pre_frame))
                                                                     (fun
-                                                                    uu___3 ->
+                                                                    uu___7 ->
                                                                     (fun
                                                                     pre_body
                                                                     ->
@@ -1001,24 +1160,24 @@ let (check :
                                                                     (Obj.magic
                                                                     (FStar_Range.mk_range
                                                                     "Pulse.Checker.WithInv.fst"
-                                                                    (Prims.of_int (326))
+                                                                    (Prims.of_int (330))
                                                                     (Prims.of_int (59))
-                                                                    (Prims.of_int (326))
+                                                                    (Prims.of_int (330))
                                                                     (Prims.of_int (67)))))
                                                                     (FStar_Sealed.seal
                                                                     (Obj.magic
                                                                     (FStar_Range.mk_range
                                                                     "Pulse.Checker.WithInv.fst"
-                                                                    (Prims.of_int (326))
+                                                                    (Prims.of_int (330))
                                                                     (Prims.of_int (70))
-                                                                    (Prims.of_int (469))
+                                                                    (Prims.of_int (473))
                                                                     (Prims.of_int (59)))))
                                                                     (FStar_Tactics_Effect.lift_div_tac
                                                                     (fun
-                                                                    uu___3 ->
+                                                                    uu___7 ->
                                                                     ()))
                                                                     (fun
-                                                                    uu___3 ->
+                                                                    uu___7 ->
                                                                     (fun
                                                                     pre_body_typing
                                                                     ->
@@ -1028,25 +1187,25 @@ let (check :
                                                                     (Obj.magic
                                                                     (FStar_Range.mk_range
                                                                     "Pulse.Checker.WithInv.fst"
-                                                                    (Prims.of_int (328))
+                                                                    (Prims.of_int (332))
                                                                     (Prims.of_int (12))
-                                                                    (Prims.of_int (328))
+                                                                    (Prims.of_int (332))
                                                                     (Prims.of_int (19)))))
                                                                     (FStar_Sealed.seal
                                                                     (Obj.magic
                                                                     (FStar_Range.mk_range
                                                                     "Pulse.Checker.WithInv.fst"
-                                                                    (Prims.of_int (329))
+                                                                    (Prims.of_int (333))
                                                                     (Prims.of_int (53))
-                                                                    (Prims.of_int (469))
+                                                                    (Prims.of_int (473))
                                                                     (Prims.of_int (59)))))
                                                                     (FStar_Tactics_Effect.lift_div_tac
                                                                     (fun
-                                                                    uu___3 ->
+                                                                    uu___7 ->
                                                                     Pulse_Typing_Env.fresh
                                                                     g))
                                                                     (fun
-                                                                    uu___3 ->
+                                                                    uu___7 ->
                                                                     (fun x ->
                                                                     Obj.magic
                                                                     (FStar_Tactics_Effect.tac_bind
@@ -1054,27 +1213,27 @@ let (check :
                                                                     (Obj.magic
                                                                     (FStar_Range.mk_range
                                                                     "Pulse.Checker.WithInv.fst"
-                                                                    (Prims.of_int (330))
+                                                                    (Prims.of_int (334))
                                                                     (Prims.of_int (13))
-                                                                    (Prims.of_int (330))
+                                                                    (Prims.of_int (334))
                                                                     (Prims.of_int (63)))))
                                                                     (FStar_Sealed.seal
                                                                     (Obj.magic
                                                                     (FStar_Range.mk_range
                                                                     "Pulse.Checker.WithInv.fst"
-                                                                    (Prims.of_int (330))
+                                                                    (Prims.of_int (334))
                                                                     (Prims.of_int (66))
-                                                                    (Prims.of_int (469))
+                                                                    (Prims.of_int (473))
                                                                     (Prims.of_int (59)))))
                                                                     (FStar_Tactics_Effect.lift_div_tac
                                                                     (fun
-                                                                    uu___3 ->
+                                                                    uu___7 ->
                                                                     Pulse_Typing_Env.push_binding
                                                                     g x
                                                                     Pulse_Syntax_Base.ppname_default
                                                                     post_hint1.Pulse_Typing.ret_ty))
                                                                     (fun
-                                                                    uu___3 ->
+                                                                    uu___7 ->
                                                                     (fun g'
                                                                     ->
                                                                     Obj.magic
@@ -1083,17 +1242,17 @@ let (check :
                                                                     (Obj.magic
                                                                     (FStar_Range.mk_range
                                                                     "Pulse.Checker.WithInv.fst"
-                                                                    (Prims.of_int (332))
+                                                                    (Prims.of_int (336))
                                                                     (Prims.of_int (53))
-                                                                    (Prims.of_int (332))
+                                                                    (Prims.of_int (336))
                                                                     (Prims.of_int (63)))))
                                                                     (FStar_Sealed.seal
                                                                     (Obj.magic
                                                                     (FStar_Range.mk_range
                                                                     "Pulse.Checker.WithInv.fst"
-                                                                    (Prims.of_int (332))
+                                                                    (Prims.of_int (336))
                                                                     (Prims.of_int (66))
-                                                                    (Prims.of_int (469))
+                                                                    (Prims.of_int (473))
                                                                     (Prims.of_int (59)))))
                                                                     (Obj.magic
                                                                     (recheck
@@ -1103,7 +1262,7 @@ let (check :
                                                                     post_hint1.Pulse_Typing.u)
                                                                     ()))
                                                                     (fun
-                                                                    uu___3 ->
+                                                                    uu___7 ->
                                                                     (fun
                                                                     post_hint_ret_ty_typing
                                                                     ->
@@ -1113,17 +1272,17 @@ let (check :
                                                                     (Obj.magic
                                                                     (FStar_Range.mk_range
                                                                     "Pulse.Checker.WithInv.fst"
-                                                                    (Prims.of_int (337))
+                                                                    (Prims.of_int (341))
                                                                     (Prims.of_int (8))
-                                                                    (Prims.of_int (337))
+                                                                    (Prims.of_int (341))
                                                                     (Prims.of_int (18)))))
                                                                     (FStar_Sealed.seal
                                                                     (Obj.magic
                                                                     (FStar_Range.mk_range
                                                                     "Pulse.Checker.WithInv.fst"
-                                                                    (Prims.of_int (338))
+                                                                    (Prims.of_int (342))
                                                                     (Prims.of_int (6))
-                                                                    (Prims.of_int (469))
+                                                                    (Prims.of_int (473))
                                                                     (Prims.of_int (59)))))
                                                                     (Obj.magic
                                                                     (recheck
@@ -1135,7 +1294,7 @@ let (check :
                                                                     Pulse_Syntax_Pure.tm_vprop
                                                                     ()))
                                                                     (fun
-                                                                    uu___3 ->
+                                                                    uu___7 ->
                                                                     (fun
                                                                     post_hint_post_typing
                                                                     ->
@@ -1145,17 +1304,17 @@ let (check :
                                                                     (Obj.magic
                                                                     (FStar_Range.mk_range
                                                                     "Pulse.Checker.WithInv.fst"
-                                                                    (Prims.of_int (340))
+                                                                    (Prims.of_int (344))
                                                                     (Prims.of_int (14))
-                                                                    (Prims.of_int (347))
+                                                                    (Prims.of_int (351))
                                                                     (Prims.of_int (7)))))
                                                                     (FStar_Sealed.seal
                                                                     (Obj.magic
                                                                     (FStar_Range.mk_range
                                                                     "Pulse.Checker.WithInv.fst"
-                                                                    (Prims.of_int (349))
+                                                                    (Prims.of_int (353))
                                                                     (Prims.of_int (4))
-                                                                    (Prims.of_int (469))
+                                                                    (Prims.of_int (473))
                                                                     (Prims.of_int (59)))))
                                                                     (Obj.magic
                                                                     (find_inv_post
@@ -1163,9 +1322,9 @@ let (check :
                                                                     post_hint1.Pulse_Typing.u
                                                                     post_hint1.Pulse_Typing.ret_ty
                                                                     post_hint1.Pulse_Typing.post
-                                                                    () () i))
+                                                                    () () i2))
                                                                     (fun
-                                                                    uu___3 ->
+                                                                    uu___7 ->
                                                                     (fun res1
                                                                     ->
                                                                     Obj.magic
@@ -1174,17 +1333,17 @@ let (check :
                                                                     (Obj.magic
                                                                     (FStar_Range.mk_range
                                                                     "Pulse.Checker.WithInv.fst"
-                                                                    (Prims.of_int (349))
+                                                                    (Prims.of_int (353))
                                                                     (Prims.of_int (4))
-                                                                    (Prims.of_int (349))
+                                                                    (Prims.of_int (353))
                                                                     (Prims.of_int (82)))))
                                                                     (FStar_Sealed.seal
                                                                     (Obj.magic
                                                                     (FStar_Range.mk_range
                                                                     "Pulse.Checker.WithInv.fst"
-                                                                    (Prims.of_int (349))
+                                                                    (Prims.of_int (353))
                                                                     (Prims.of_int (83))
-                                                                    (Prims.of_int (469))
+                                                                    (Prims.of_int (473))
                                                                     (Prims.of_int (59)))))
                                                                     (if
                                                                     FStar_Pervasives_Native.uu___is_None
@@ -1202,46 +1361,46 @@ let (check :
                                                                     (Obj.repr
                                                                     (FStar_Tactics_Effect.lift_div_tac
                                                                     (fun
-                                                                    uu___4 ->
+                                                                    uu___8 ->
                                                                     ()))))
                                                                     (fun
-                                                                    uu___3 ->
+                                                                    uu___7 ->
                                                                     (fun
-                                                                    uu___3 ->
+                                                                    uu___7 ->
                                                                     Obj.magic
                                                                     (FStar_Tactics_Effect.tac_bind
                                                                     (FStar_Sealed.seal
                                                                     (Obj.magic
                                                                     (FStar_Range.mk_range
                                                                     "Pulse.Checker.WithInv.fst"
-                                                                    (Prims.of_int (351))
+                                                                    (Prims.of_int (355))
                                                                     (Prims.of_int (78))
-                                                                    (Prims.of_int (351))
+                                                                    (Prims.of_int (355))
                                                                     (Prims.of_int (81)))))
                                                                     (FStar_Sealed.seal
                                                                     (Obj.magic
                                                                     (FStar_Range.mk_range
                                                                     "Pulse.Checker.WithInv.fst"
-                                                                    (Prims.of_int (349))
+                                                                    (Prims.of_int (353))
                                                                     (Prims.of_int (83))
-                                                                    (Prims.of_int (469))
+                                                                    (Prims.of_int (473))
                                                                     (Prims.of_int (59)))))
                                                                     (FStar_Tactics_Effect.lift_div_tac
                                                                     (fun
-                                                                    uu___4 ->
+                                                                    uu___8 ->
                                                                     res1))
                                                                     (fun
-                                                                    uu___4 ->
+                                                                    uu___8 ->
                                                                     (fun
-                                                                    uu___4 ->
-                                                                    match uu___4
+                                                                    uu___8 ->
+                                                                    match uu___8
                                                                     with
                                                                     | 
                                                                     FStar_Pervasives_Native.Some
                                                                     (FStar_Pervasives.Mkdtuple5
                                                                     (p',
                                                                     post_frame,
-                                                                    uu___5,
+                                                                    uu___9,
                                                                     post_frame_typing,
                                                                     d_post_frame_equiv))
                                                                     ->
@@ -1251,26 +1410,28 @@ let (check :
                                                                     (Obj.magic
                                                                     (FStar_Range.mk_range
                                                                     "Pulse.Checker.WithInv.fst"
-                                                                    (Prims.of_int (354))
+                                                                    (Prims.of_int (358))
                                                                     (Prims.of_int (20))
-                                                                    (Prims.of_int (354))
+                                                                    (Prims.of_int (358))
                                                                     (Prims.of_int (40)))))
                                                                     (FStar_Sealed.seal
                                                                     (Obj.magic
                                                                     (FStar_Range.mk_range
                                                                     "Pulse.Checker.WithInv.fst"
-                                                                    (Prims.of_int (354))
+                                                                    (Prims.of_int (358))
                                                                     (Prims.of_int (43))
-                                                                    (Prims.of_int (469))
+                                                                    (Prims.of_int (473))
                                                                     (Prims.of_int (59)))))
                                                                     (FStar_Tactics_Effect.lift_div_tac
                                                                     (fun
-                                                                    uu___6 ->
+                                                                    uu___10
+                                                                    ->
                                                                     Pulse_Syntax_Pure.tm_star
                                                                     p
                                                                     post_frame))
                                                                     (fun
-                                                                    uu___6 ->
+                                                                    uu___10
+                                                                    ->
                                                                     (fun
                                                                     post_body
                                                                     ->
@@ -1280,21 +1441,22 @@ let (check :
                                                                     (Obj.magic
                                                                     (FStar_Range.mk_range
                                                                     "Pulse.Checker.WithInv.fst"
-                                                                    (Prims.of_int (358))
+                                                                    (Prims.of_int (362))
                                                                     (Prims.of_int (8))
-                                                                    (Prims.of_int (363))
+                                                                    (Prims.of_int (367))
                                                                     (Prims.of_int (75)))))
                                                                     (FStar_Sealed.seal
                                                                     (Obj.magic
                                                                     (FStar_Range.mk_range
                                                                     "Pulse.Checker.WithInv.fst"
-                                                                    (Prims.of_int (354))
+                                                                    (Prims.of_int (358))
                                                                     (Prims.of_int (43))
-                                                                    (Prims.of_int (469))
+                                                                    (Prims.of_int (473))
                                                                     (Prims.of_int (59)))))
                                                                     (FStar_Tactics_Effect.lift_div_tac
                                                                     (fun
-                                                                    uu___6 ->
+                                                                    uu___10
+                                                                    ->
                                                                     match 
                                                                     post_hint1.Pulse_Typing.effect_annot
                                                                     with
@@ -1323,10 +1485,12 @@ let (check :
                                                                     (opens,
                                                                     ())))
                                                                     (fun
-                                                                    uu___6 ->
+                                                                    uu___10
+                                                                    ->
                                                                     (fun
-                                                                    uu___6 ->
-                                                                    match uu___6
+                                                                    uu___10
+                                                                    ->
+                                                                    match uu___10
                                                                     with
                                                                     | 
                                                                     Prims.Mkdtuple2
@@ -1339,51 +1503,56 @@ let (check :
                                                                     (Obj.magic
                                                                     (FStar_Range.mk_range
                                                                     "Pulse.Checker.WithInv.fst"
-                                                                    (Prims.of_int (364))
+                                                                    (Prims.of_int (368))
                                                                     (Prims.of_int (6))
-                                                                    (Prims.of_int (469))
+                                                                    (Prims.of_int (473))
                                                                     (Prims.of_int (59)))))
                                                                     (FStar_Sealed.seal
                                                                     (Obj.magic
                                                                     (FStar_Range.mk_range
                                                                     "Pulse.Checker.WithInv.fst"
-                                                                    (Prims.of_int (364))
+                                                                    (Prims.of_int (368))
                                                                     (Prims.of_int (6))
-                                                                    (Prims.of_int (469))
+                                                                    (Prims.of_int (473))
                                                                     (Prims.of_int (59)))))
                                                                     (FStar_Tactics_Effect.lift_div_tac
                                                                     (fun
-                                                                    uu___7 ->
-                                                                    uu___6))
+                                                                    uu___11
+                                                                    ->
+                                                                    uu___10))
                                                                     (fun
-                                                                    uu___7 ->
+                                                                    uu___11
+                                                                    ->
                                                                     (fun
-                                                                    uu___7 ->
+                                                                    uu___11
+                                                                    ->
                                                                     Obj.magic
                                                                     (FStar_Tactics_Effect.tac_bind
                                                                     (FStar_Sealed.seal
                                                                     (Obj.magic
                                                                     (FStar_Range.mk_range
                                                                     "Pulse.Checker.WithInv.fst"
-                                                                    (Prims.of_int (365))
+                                                                    (Prims.of_int (369))
                                                                     (Prims.of_int (25))
-                                                                    (Prims.of_int (365))
+                                                                    (Prims.of_int (369))
                                                                     (Prims.of_int (45)))))
                                                                     (FStar_Sealed.seal
                                                                     (Obj.magic
                                                                     (FStar_Range.mk_range
                                                                     "Pulse.Checker.WithInv.fst"
-                                                                    (Prims.of_int (365))
+                                                                    (Prims.of_int (369))
                                                                     (Prims.of_int (48))
-                                                                    (Prims.of_int (469))
+                                                                    (Prims.of_int (473))
                                                                     (Prims.of_int (59)))))
                                                                     (FStar_Tactics_Effect.lift_div_tac
                                                                     (fun
-                                                                    uu___8 ->
+                                                                    uu___12
+                                                                    ->
                                                                     remove_iname
-                                                                    opens i))
+                                                                    opens i2))
                                                                     (fun
-                                                                    uu___8 ->
+                                                                    uu___12
+                                                                    ->
                                                                     (fun
                                                                     opens_remove_i
                                                                     ->
@@ -1393,21 +1562,22 @@ let (check :
                                                                     (Obj.magic
                                                                     (FStar_Range.mk_range
                                                                     "Pulse.Checker.WithInv.fst"
-                                                                    (Prims.of_int (367))
+                                                                    (Prims.of_int (371))
                                                                     (Prims.of_int (6))
-                                                                    (Prims.of_int (372))
+                                                                    (Prims.of_int (376))
                                                                     (Prims.of_int (49)))))
                                                                     (FStar_Sealed.seal
                                                                     (Obj.magic
                                                                     (FStar_Range.mk_range
                                                                     "Pulse.Checker.WithInv.fst"
-                                                                    (Prims.of_int (372))
+                                                                    (Prims.of_int (376))
                                                                     (Prims.of_int (52))
-                                                                    (Prims.of_int (469))
+                                                                    (Prims.of_int (473))
                                                                     (Prims.of_int (59)))))
                                                                     (FStar_Tactics_Effect.lift_div_tac
                                                                     (fun
-                                                                    uu___8 ->
+                                                                    uu___12
+                                                                    ->
                                                                     match 
                                                                     post_hint1.Pulse_Typing.effect_annot
                                                                     with
@@ -1422,7 +1592,8 @@ let (check :
                                                                     }
                                                                     | 
                                                                     Pulse_Syntax_Base.EffectAnnotAtomic
-                                                                    uu___9 ->
+                                                                    uu___13
+                                                                    ->
                                                                     Pulse_Syntax_Base.EffectAnnotAtomic
                                                                     {
                                                                     Pulse_Syntax_Base.opens1
@@ -1431,7 +1602,8 @@ let (check :
                                                                     }
                                                                     | 
                                                                     Pulse_Syntax_Base.EffectAnnotGhost
-                                                                    uu___9 ->
+                                                                    uu___13
+                                                                    ->
                                                                     Pulse_Syntax_Base.EffectAnnotGhost
                                                                     {
                                                                     Pulse_Syntax_Base.opens
@@ -1439,7 +1611,8 @@ let (check :
                                                                     opens_remove_i
                                                                     }))
                                                                     (fun
-                                                                    uu___8 ->
+                                                                    uu___12
+                                                                    ->
                                                                     (fun
                                                                     effect_annot
                                                                     ->
@@ -1449,28 +1622,31 @@ let (check :
                                                                     (Obj.magic
                                                                     (FStar_Range.mk_range
                                                                     "Pulse.Checker.WithInv.fst"
-                                                                    (Prims.of_int (375))
+                                                                    (Prims.of_int (379))
                                                                     (Prims.of_int (8))
-                                                                    (Prims.of_int (375))
+                                                                    (Prims.of_int (379))
                                                                     (Prims.of_int (63)))))
                                                                     (FStar_Sealed.seal
                                                                     (Obj.magic
                                                                     (FStar_Range.mk_range
                                                                     "Pulse.Checker.WithInv.fst"
-                                                                    (Prims.of_int (378))
+                                                                    (Prims.of_int (382))
                                                                     (Prims.of_int (48))
-                                                                    (Prims.of_int (469))
+                                                                    (Prims.of_int (473))
                                                                     (Prims.of_int (59)))))
                                                                     (FStar_Tactics_Effect.lift_div_tac
                                                                     (fun
-                                                                    uu___8 ->
+                                                                    uu___12
+                                                                    ->
                                                                     (fun
-                                                                    uu___8 ->
+                                                                    uu___12
+                                                                    ->
                                                                     Obj.magic
                                                                     ())
-                                                                    uu___8))
+                                                                    uu___12))
                                                                     (fun
-                                                                    uu___8 ->
+                                                                    uu___12
+                                                                    ->
                                                                     (fun
                                                                     effect_annot_typing
                                                                     ->
@@ -1480,21 +1656,22 @@ let (check :
                                                                     (Obj.magic
                                                                     (FStar_Range.mk_range
                                                                     "Pulse.Checker.WithInv.fst"
-                                                                    (Prims.of_int (379))
+                                                                    (Prims.of_int (383))
                                                                     (Prims.of_int (50))
-                                                                    (Prims.of_int (387))
+                                                                    (Prims.of_int (391))
                                                                     (Prims.of_int (27)))))
                                                                     (FStar_Sealed.seal
                                                                     (Obj.magic
                                                                     (FStar_Range.mk_range
                                                                     "Pulse.Checker.WithInv.fst"
-                                                                    (Prims.of_int (388))
+                                                                    (Prims.of_int (392))
                                                                     (Prims.of_int (8))
-                                                                    (Prims.of_int (469))
+                                                                    (Prims.of_int (473))
                                                                     (Prims.of_int (59)))))
                                                                     (FStar_Tactics_Effect.lift_div_tac
                                                                     (fun
-                                                                    uu___8 ->
+                                                                    uu___12
+                                                                    ->
                                                                     {
                                                                     Pulse_Typing.g
                                                                     = g;
@@ -1523,7 +1700,8 @@ let (check :
                                                                     = ()
                                                                     }))
                                                                     (fun
-                                                                    uu___8 ->
+                                                                    uu___12
+                                                                    ->
                                                                     (fun
                                                                     post_hint_body
                                                                     ->
@@ -1533,17 +1711,17 @@ let (check :
                                                                     (Obj.magic
                                                                     (FStar_Range.mk_range
                                                                     "Pulse.Checker.WithInv.fst"
-                                                                    (Prims.of_int (390))
+                                                                    (Prims.of_int (394))
                                                                     (Prims.of_int (41))
-                                                                    (Prims.of_int (393))
+                                                                    (Prims.of_int (397))
                                                                     (Prims.of_int (37)))))
                                                                     (FStar_Sealed.seal
                                                                     (Obj.magic
                                                                     (FStar_Range.mk_range
                                                                     "Pulse.Checker.WithInv.fst"
-                                                                    (Prims.of_int (388))
+                                                                    (Prims.of_int (392))
                                                                     (Prims.of_int (8))
-                                                                    (Prims.of_int (469))
+                                                                    (Prims.of_int (473))
                                                                     (Prims.of_int (59)))))
                                                                     (Obj.magic
                                                                     (FStar_Tactics_Effect.tac_bind
@@ -1551,25 +1729,27 @@ let (check :
                                                                     (Obj.magic
                                                                     (FStar_Range.mk_range
                                                                     "Pulse.Checker.WithInv.fst"
-                                                                    (Prims.of_int (391))
+                                                                    (Prims.of_int (395))
                                                                     (Prims.of_int (19))
-                                                                    (Prims.of_int (391))
+                                                                    (Prims.of_int (395))
                                                                     (Prims.of_int (53)))))
                                                                     (FStar_Sealed.seal
                                                                     (Obj.magic
                                                                     (FStar_Range.mk_range
                                                                     "Pulse.Checker.WithInv.fst"
-                                                                    (Prims.of_int (391))
+                                                                    (Prims.of_int (395))
                                                                     (Prims.of_int (56))
-                                                                    (Prims.of_int (393))
+                                                                    (Prims.of_int (397))
                                                                     (Prims.of_int (37)))))
                                                                     (FStar_Tactics_Effect.lift_div_tac
                                                                     (fun
-                                                                    uu___8 ->
+                                                                    uu___12
+                                                                    ->
                                                                     Pulse_Syntax_Base.mk_ppname_no_range
                                                                     "with_inv_body"))
                                                                     (fun
-                                                                    uu___8 ->
+                                                                    uu___12
+                                                                    ->
                                                                     (fun
                                                                     ppname ->
                                                                     Obj.magic
@@ -1578,17 +1758,17 @@ let (check :
                                                                     (Obj.magic
                                                                     (FStar_Range.mk_range
                                                                     "Pulse.Checker.WithInv.fst"
-                                                                    (Prims.of_int (392))
+                                                                    (Prims.of_int (396))
                                                                     (Prims.of_int (14))
-                                                                    (Prims.of_int (392))
+                                                                    (Prims.of_int (396))
                                                                     (Prims.of_int (80)))))
                                                                     (FStar_Sealed.seal
                                                                     (Obj.magic
                                                                     (FStar_Range.mk_range
                                                                     "Pulse.Checker.WithInv.fst"
-                                                                    (Prims.of_int (393))
+                                                                    (Prims.of_int (397))
                                                                     (Prims.of_int (6))
-                                                                    (Prims.of_int (393))
+                                                                    (Prims.of_int (397))
                                                                     (Prims.of_int (37)))))
                                                                     (Obj.magic
                                                                     (check1 g
@@ -1599,7 +1779,8 @@ let (check :
                                                                     ppname
                                                                     body))
                                                                     (fun
-                                                                    uu___8 ->
+                                                                    uu___12
+                                                                    ->
                                                                     (fun r ->
                                                                     Obj.magic
                                                                     (Pulse_Checker_Base.apply_checker_result_k
@@ -1607,13 +1788,15 @@ let (check :
                                                                     pre_body
                                                                     post_hint_body
                                                                     r ppname))
-                                                                    uu___8)))
-                                                                    uu___8)))
+                                                                    uu___12)))
+                                                                    uu___12)))
                                                                     (fun
-                                                                    uu___8 ->
+                                                                    uu___12
+                                                                    ->
                                                                     (fun
-                                                                    uu___8 ->
-                                                                    match uu___8
+                                                                    uu___12
+                                                                    ->
+                                                                    match uu___12
                                                                     with
                                                                     | 
                                                                     FStar_Pervasives.Mkdtuple3
@@ -1627,30 +1810,32 @@ let (check :
                                                                     (Obj.magic
                                                                     (FStar_Range.mk_range
                                                                     "Pulse.Checker.WithInv.fst"
-                                                                    (Prims.of_int (400))
+                                                                    (Prims.of_int (404))
                                                                     (Prims.of_int (16))
-                                                                    (Prims.of_int (403))
+                                                                    (Prims.of_int (407))
                                                                     (Prims.of_int (20)))))
                                                                     (FStar_Sealed.seal
                                                                     (Obj.magic
                                                                     (FStar_Range.mk_range
                                                                     "Pulse.Checker.WithInv.fst"
-                                                                    (Prims.of_int (403))
+                                                                    (Prims.of_int (407))
                                                                     (Prims.of_int (23))
-                                                                    (Prims.of_int (469))
+                                                                    (Prims.of_int (473))
                                                                     (Prims.of_int (59)))))
                                                                     (FStar_Tactics_Effect.lift_div_tac
                                                                     (fun
-                                                                    uu___9 ->
+                                                                    uu___13
+                                                                    ->
                                                                     atomic_or_ghost_with_inames_and_pre_post
                                                                     c_body
                                                                     (Pulse_Reflection_Util.add_inv_tm
                                                                     (Pulse_Syntax_Base.comp_inames
-                                                                    c_body) i)
-                                                                    pre
+                                                                    c_body)
+                                                                    i2) pre
                                                                     post_hint1.Pulse_Typing.post))
                                                                     (fun
-                                                                    uu___9 ->
+                                                                    uu___13
+                                                                    ->
                                                                     (fun
                                                                     c_out ->
                                                                     Obj.magic
@@ -1659,23 +1844,25 @@ let (check :
                                                                     (Obj.magic
                                                                     (FStar_Range.mk_range
                                                                     "Pulse.Checker.WithInv.fst"
-                                                                    (Prims.of_int (405))
+                                                                    (Prims.of_int (409))
                                                                     (Prims.of_int (14))
-                                                                    (Prims.of_int (405))
+                                                                    (Prims.of_int (409))
                                                                     (Prims.of_int (47)))))
                                                                     (FStar_Sealed.seal
                                                                     (Obj.magic
                                                                     (FStar_Range.mk_range
                                                                     "Pulse.Checker.WithInv.fst"
-                                                                    (Prims.of_int (405))
+                                                                    (Prims.of_int (409))
                                                                     (Prims.of_int (50))
-                                                                    (Prims.of_int (469))
+                                                                    (Prims.of_int (473))
                                                                     (Prims.of_int (59)))))
                                                                     (Obj.magic
                                                                     (disjointness_remove_i_i
-                                                                    g opens i))
+                                                                    g opens
+                                                                    i2))
                                                                     (fun
-                                                                    uu___9 ->
+                                                                    uu___13
+                                                                    ->
                                                                     (fun tok
                                                                     ->
                                                                     Obj.magic
@@ -1684,21 +1871,22 @@ let (check :
                                                                     (Obj.magic
                                                                     (FStar_Range.mk_range
                                                                     "Pulse.Checker.WithInv.fst"
-                                                                    (Prims.of_int (407))
+                                                                    (Prims.of_int (411))
                                                                     (Prims.of_int (13))
-                                                                    (Prims.of_int (407))
+                                                                    (Prims.of_int (411))
                                                                     (Prims.of_int (92)))))
                                                                     (FStar_Sealed.seal
                                                                     (Obj.magic
                                                                     (FStar_Range.mk_range
                                                                     "Pulse.Checker.WithInv.fst"
-                                                                    (Prims.of_int (407))
+                                                                    (Prims.of_int (411))
                                                                     (Prims.of_int (95))
-                                                                    (Prims.of_int (469))
+                                                                    (Prims.of_int (473))
                                                                     (Prims.of_int (59)))))
                                                                     (FStar_Tactics_Effect.lift_div_tac
                                                                     (fun
-                                                                    uu___9 ->
+                                                                    uu___13
+                                                                    ->
                                                                     Pulse_Typing.wtag
                                                                     (FStar_Pervasives_Native.Some
                                                                     (Pulse_Syntax_Base.ctag_of_comp_st
@@ -1706,7 +1894,7 @@ let (check :
                                                                     (Pulse_Syntax_Base.Tm_WithInv
                                                                     {
                                                                     Pulse_Syntax_Base.name1
-                                                                    = i;
+                                                                    = i2;
                                                                     Pulse_Syntax_Base.body6
                                                                     = body1;
                                                                     Pulse_Syntax_Base.returns_inv
@@ -1714,7 +1902,8 @@ let (check :
                                                                     FStar_Pervasives_Native.None
                                                                     })))
                                                                     (fun
-                                                                    uu___9 ->
+                                                                    uu___13
+                                                                    ->
                                                                     (fun tm
                                                                     ->
                                                                     Obj.magic
@@ -1723,21 +1912,22 @@ let (check :
                                                                     (Obj.magic
                                                                     (FStar_Range.mk_range
                                                                     "Pulse.Checker.WithInv.fst"
-                                                                    (Prims.of_int (408))
+                                                                    (Prims.of_int (412))
                                                                     (Prims.of_int (34))
-                                                                    (Prims.of_int (447))
+                                                                    (Prims.of_int (451))
                                                                     (Prims.of_int (7)))))
                                                                     (FStar_Sealed.seal
                                                                     (Obj.magic
                                                                     (FStar_Range.mk_range
                                                                     "Pulse.Checker.WithInv.fst"
-                                                                    (Prims.of_int (449))
+                                                                    (Prims.of_int (453))
                                                                     (Prims.of_int (4))
-                                                                    (Prims.of_int (469))
+                                                                    (Prims.of_int (473))
                                                                     (Prims.of_int (59)))))
                                                                     (FStar_Tactics_Effect.lift_div_tac
                                                                     (fun
-                                                                    uu___9 ->
+                                                                    uu___13
+                                                                    ->
                                                                     Pulse_Typing.T_Equiv
                                                                     (g,
                                                                     (Pulse_Typing.wtag
@@ -1752,7 +1942,7 @@ let (check :
                                                                     (Pulse_Syntax_Base.Tm_WithInv
                                                                     {
                                                                     Pulse_Syntax_Base.name1
-                                                                    = i;
+                                                                    = i2;
                                                                     Pulse_Syntax_Base.body6
                                                                     = body1;
                                                                     Pulse_Syntax_Base.returns_inv
@@ -1763,19 +1953,20 @@ let (check :
                                                                     c_body
                                                                     (Pulse_Reflection_Util.add_inv_tm
                                                                     (Pulse_Syntax_Base.comp_inames
-                                                                    c_body) i)
+                                                                    c_body)
+                                                                    i2)
                                                                     (Pulse_Syntax_Pure.tm_star
                                                                     (Pulse_Syntax_Pure.tm_inv
-                                                                    i p)
+                                                                    i2 p)
                                                                     pre_frame)
                                                                     (Pulse_Syntax_Pure.tm_star
                                                                     (Pulse_Syntax_Pure.tm_inv
-                                                                    i p)
+                                                                    i2 p)
                                                                     post_frame)),
                                                                     c_out,
                                                                     (Pulse_Typing.T_WithInv
-                                                                    (g, i, p,
-                                                                    body1,
+                                                                    (g, i2,
+                                                                    p, body1,
                                                                     (atomic_or_ghost_with_inames_and_pre_post
                                                                     c_body
                                                                     (Pulse_Syntax_Base.comp_inames
@@ -1791,14 +1982,15 @@ let (check :
                                                                     c_body
                                                                     (Pulse_Reflection_Util.add_inv_tm
                                                                     (Pulse_Syntax_Base.comp_inames
-                                                                    c_body) i)
+                                                                    c_body)
+                                                                    i2)
                                                                     (Pulse_Syntax_Pure.tm_star
                                                                     (Pulse_Syntax_Pure.tm_inv
-                                                                    i p)
+                                                                    i2 p)
                                                                     pre_frame)
                                                                     (Pulse_Syntax_Pure.tm_star
                                                                     (Pulse_Syntax_Pure.tm_inv
-                                                                    i p)
+                                                                    i2 p)
                                                                     post_frame)),
                                                                     c_out, x,
                                                                     (), (),
@@ -1812,50 +2004,53 @@ let (check :
                                                                     c_body
                                                                     (Pulse_Reflection_Util.add_inv_tm
                                                                     (Pulse_Syntax_Base.comp_inames
-                                                                    c_body) i)
+                                                                    c_body)
+                                                                    i2)
                                                                     (Pulse_Syntax_Pure.tm_star
                                                                     (Pulse_Syntax_Pure.tm_inv
-                                                                    i p)
+                                                                    i2 p)
                                                                     pre_frame)
                                                                     (Pulse_Syntax_Pure.tm_star
                                                                     (Pulse_Syntax_Pure.tm_inv
-                                                                    i p)
+                                                                    i2 p)
                                                                     post_frame)))),
                                                                     FStar_Reflection_Typing.R_Eq)),
                                                                     (), ())))))
                                                                     (fun
-                                                                    uu___9 ->
+                                                                    uu___13
+                                                                    ->
                                                                     (fun d ->
                                                                     match 
                                                                     post_hint1.Pulse_Typing.effect_annot
                                                                     with
                                                                     | 
                                                                     Pulse_Syntax_Base.EffectAnnotGhost
-                                                                    uu___9 ->
+                                                                    uu___13
+                                                                    ->
                                                                     Obj.magic
                                                                     (FStar_Tactics_Effect.tac_bind
                                                                     (FStar_Sealed.seal
                                                                     (Obj.magic
                                                                     (FStar_Range.mk_range
                                                                     "Pulse.Checker.WithInv.fst"
-                                                                    (Prims.of_int (453))
+                                                                    (Prims.of_int (457))
                                                                     (Prims.of_int (8))
-                                                                    (Prims.of_int (453))
+                                                                    (Prims.of_int (457))
                                                                     (Prims.of_int (60)))))
                                                                     (FStar_Sealed.seal
                                                                     (Obj.magic
                                                                     (FStar_Range.mk_range
                                                                     "Pulse.Checker.WithInv.fst"
-                                                                    (Prims.of_int (454))
+                                                                    (Prims.of_int (458))
                                                                     (Prims.of_int (8))
-                                                                    (Prims.of_int (465))
+                                                                    (Prims.of_int (469))
                                                                     (Prims.of_int (59)))))
                                                                     (Obj.magic
                                                                     (add_remove_inverse
-                                                                    g opens i
-                                                                    () ()))
+                                                                    g opens
+                                                                    i2 () ()))
                                                                     (fun
-                                                                    uu___10
+                                                                    uu___14
                                                                     ->
                                                                     (fun tok1
                                                                     ->
@@ -1865,21 +2060,21 @@ let (check :
                                                                     (Obj.magic
                                                                     (FStar_Range.mk_range
                                                                     "Pulse.Checker.WithInv.fst"
-                                                                    (Prims.of_int (456))
+                                                                    (Prims.of_int (460))
                                                                     (Prims.of_int (8))
-                                                                    (Prims.of_int (462))
+                                                                    (Prims.of_int (466))
                                                                     (Prims.of_int (51)))))
                                                                     (FStar_Sealed.seal
                                                                     (Obj.magic
                                                                     (FStar_Range.mk_range
                                                                     "Pulse.Checker.WithInv.fst"
-                                                                    (Prims.of_int (454))
+                                                                    (Prims.of_int (458))
                                                                     (Prims.of_int (8))
-                                                                    (Prims.of_int (465))
+                                                                    (Prims.of_int (469))
                                                                     (Prims.of_int (59)))))
                                                                     (FStar_Tactics_Effect.lift_div_tac
                                                                     (fun
-                                                                    uu___10
+                                                                    uu___14
                                                                     ->
                                                                     match c_out
                                                                     with
@@ -1912,12 +2107,12 @@ let (check :
                                                                     opens,
                                                                     ())))))
                                                                     (fun
-                                                                    uu___10
+                                                                    uu___14
                                                                     ->
                                                                     (fun
-                                                                    uu___10
+                                                                    uu___14
                                                                     ->
-                                                                    match uu___10
+                                                                    match uu___14
                                                                     with
                                                                     | 
                                                                     Prims.Mkdtuple2
@@ -1930,28 +2125,28 @@ let (check :
                                                                     (Obj.magic
                                                                     (FStar_Range.mk_range
                                                                     "Pulse.Checker.WithInv.fst"
-                                                                    (Prims.of_int (462))
+                                                                    (Prims.of_int (466))
                                                                     (Prims.of_int (54))
-                                                                    (Prims.of_int (465))
+                                                                    (Prims.of_int (469))
                                                                     (Prims.of_int (59)))))
                                                                     (FStar_Sealed.seal
                                                                     (Obj.magic
                                                                     (FStar_Range.mk_range
                                                                     "Pulse.Checker.WithInv.fst"
-                                                                    (Prims.of_int (462))
+                                                                    (Prims.of_int (466))
                                                                     (Prims.of_int (54))
-                                                                    (Prims.of_int (465))
+                                                                    (Prims.of_int (469))
                                                                     (Prims.of_int (59)))))
                                                                     (FStar_Tactics_Effect.lift_div_tac
                                                                     (fun
-                                                                    uu___11
+                                                                    uu___15
                                                                     ->
-                                                                    uu___10))
+                                                                    uu___14))
                                                                     (fun
-                                                                    uu___11
+                                                                    uu___15
                                                                     ->
                                                                     (fun
-                                                                    uu___11
+                                                                    uu___15
                                                                     ->
                                                                     Obj.magic
                                                                     (FStar_Tactics_Effect.tac_bind
@@ -1959,21 +2154,21 @@ let (check :
                                                                     (Obj.magic
                                                                     (FStar_Range.mk_range
                                                                     "Pulse.Checker.WithInv.fst"
-                                                                    (Prims.of_int (464))
+                                                                    (Prims.of_int (468))
                                                                     (Prims.of_int (8))
-                                                                    (Prims.of_int (464))
+                                                                    (Prims.of_int (468))
                                                                     (Prims.of_int (31)))))
                                                                     (FStar_Sealed.seal
                                                                     (Obj.magic
                                                                     (FStar_Range.mk_range
                                                                     "Pulse.Checker.WithInv.fst"
-                                                                    (Prims.of_int (465))
+                                                                    (Prims.of_int (469))
                                                                     (Prims.of_int (6))
-                                                                    (Prims.of_int (465))
+                                                                    (Prims.of_int (469))
                                                                     (Prims.of_int (59)))))
                                                                     (FStar_Tactics_Effect.lift_div_tac
                                                                     (fun
-                                                                    uu___12
+                                                                    uu___16
                                                                     ->
                                                                     Pulse_Typing.T_Sub
                                                                     (g, tm,
@@ -1982,7 +2177,7 @@ let (check :
                                                                     d,
                                                                     d_sub_c)))
                                                                     (fun
-                                                                    uu___12
+                                                                    uu___16
                                                                     ->
                                                                     (fun d1
                                                                     ->
@@ -1995,37 +2190,38 @@ let (check :
                                                                     c_out_opens,
                                                                     d1))
                                                                     res_ppname))
-                                                                    uu___12)))
-                                                                    uu___11)))
-                                                                    uu___10)))
-                                                                    uu___10))
+                                                                    uu___16)))
+                                                                    uu___15)))
+                                                                    uu___14)))
+                                                                    uu___14))
                                                                     | 
                                                                     Pulse_Syntax_Base.EffectAnnotAtomic
-                                                                    uu___9 ->
+                                                                    uu___13
+                                                                    ->
                                                                     Obj.magic
                                                                     (FStar_Tactics_Effect.tac_bind
                                                                     (FStar_Sealed.seal
                                                                     (Obj.magic
                                                                     (FStar_Range.mk_range
                                                                     "Pulse.Checker.WithInv.fst"
-                                                                    (Prims.of_int (453))
+                                                                    (Prims.of_int (457))
                                                                     (Prims.of_int (8))
-                                                                    (Prims.of_int (453))
+                                                                    (Prims.of_int (457))
                                                                     (Prims.of_int (60)))))
                                                                     (FStar_Sealed.seal
                                                                     (Obj.magic
                                                                     (FStar_Range.mk_range
                                                                     "Pulse.Checker.WithInv.fst"
-                                                                    (Prims.of_int (454))
+                                                                    (Prims.of_int (458))
                                                                     (Prims.of_int (8))
-                                                                    (Prims.of_int (465))
+                                                                    (Prims.of_int (469))
                                                                     (Prims.of_int (59)))))
                                                                     (Obj.magic
                                                                     (add_remove_inverse
-                                                                    g opens i
-                                                                    () ()))
+                                                                    g opens
+                                                                    i2 () ()))
                                                                     (fun
-                                                                    uu___10
+                                                                    uu___14
                                                                     ->
                                                                     (fun tok1
                                                                     ->
@@ -2035,21 +2231,21 @@ let (check :
                                                                     (Obj.magic
                                                                     (FStar_Range.mk_range
                                                                     "Pulse.Checker.WithInv.fst"
-                                                                    (Prims.of_int (456))
+                                                                    (Prims.of_int (460))
                                                                     (Prims.of_int (8))
-                                                                    (Prims.of_int (462))
+                                                                    (Prims.of_int (466))
                                                                     (Prims.of_int (51)))))
                                                                     (FStar_Sealed.seal
                                                                     (Obj.magic
                                                                     (FStar_Range.mk_range
                                                                     "Pulse.Checker.WithInv.fst"
-                                                                    (Prims.of_int (454))
+                                                                    (Prims.of_int (458))
                                                                     (Prims.of_int (8))
-                                                                    (Prims.of_int (465))
+                                                                    (Prims.of_int (469))
                                                                     (Prims.of_int (59)))))
                                                                     (FStar_Tactics_Effect.lift_div_tac
                                                                     (fun
-                                                                    uu___10
+                                                                    uu___14
                                                                     ->
                                                                     match c_out
                                                                     with
@@ -2082,12 +2278,12 @@ let (check :
                                                                     opens,
                                                                     ())))))
                                                                     (fun
-                                                                    uu___10
+                                                                    uu___14
                                                                     ->
                                                                     (fun
-                                                                    uu___10
+                                                                    uu___14
                                                                     ->
-                                                                    match uu___10
+                                                                    match uu___14
                                                                     with
                                                                     | 
                                                                     Prims.Mkdtuple2
@@ -2100,28 +2296,28 @@ let (check :
                                                                     (Obj.magic
                                                                     (FStar_Range.mk_range
                                                                     "Pulse.Checker.WithInv.fst"
-                                                                    (Prims.of_int (462))
+                                                                    (Prims.of_int (466))
                                                                     (Prims.of_int (54))
-                                                                    (Prims.of_int (465))
+                                                                    (Prims.of_int (469))
                                                                     (Prims.of_int (59)))))
                                                                     (FStar_Sealed.seal
                                                                     (Obj.magic
                                                                     (FStar_Range.mk_range
                                                                     "Pulse.Checker.WithInv.fst"
-                                                                    (Prims.of_int (462))
+                                                                    (Prims.of_int (466))
                                                                     (Prims.of_int (54))
-                                                                    (Prims.of_int (465))
+                                                                    (Prims.of_int (469))
                                                                     (Prims.of_int (59)))))
                                                                     (FStar_Tactics_Effect.lift_div_tac
                                                                     (fun
-                                                                    uu___11
+                                                                    uu___15
                                                                     ->
-                                                                    uu___10))
+                                                                    uu___14))
                                                                     (fun
-                                                                    uu___11
+                                                                    uu___15
                                                                     ->
                                                                     (fun
-                                                                    uu___11
+                                                                    uu___15
                                                                     ->
                                                                     Obj.magic
                                                                     (FStar_Tactics_Effect.tac_bind
@@ -2129,21 +2325,21 @@ let (check :
                                                                     (Obj.magic
                                                                     (FStar_Range.mk_range
                                                                     "Pulse.Checker.WithInv.fst"
-                                                                    (Prims.of_int (464))
+                                                                    (Prims.of_int (468))
                                                                     (Prims.of_int (8))
-                                                                    (Prims.of_int (464))
+                                                                    (Prims.of_int (468))
                                                                     (Prims.of_int (31)))))
                                                                     (FStar_Sealed.seal
                                                                     (Obj.magic
                                                                     (FStar_Range.mk_range
                                                                     "Pulse.Checker.WithInv.fst"
-                                                                    (Prims.of_int (465))
+                                                                    (Prims.of_int (469))
                                                                     (Prims.of_int (6))
-                                                                    (Prims.of_int (465))
+                                                                    (Prims.of_int (469))
                                                                     (Prims.of_int (59)))))
                                                                     (FStar_Tactics_Effect.lift_div_tac
                                                                     (fun
-                                                                    uu___12
+                                                                    uu___16
                                                                     ->
                                                                     Pulse_Typing.T_Sub
                                                                     (g, tm,
@@ -2152,7 +2348,7 @@ let (check :
                                                                     d,
                                                                     d_sub_c)))
                                                                     (fun
-                                                                    uu___12
+                                                                    uu___16
                                                                     ->
                                                                     (fun d1
                                                                     ->
@@ -2165,10 +2361,10 @@ let (check :
                                                                     c_out_opens,
                                                                     d1))
                                                                     res_ppname))
-                                                                    uu___12)))
-                                                                    uu___11)))
-                                                                    uu___10)))
-                                                                    uu___10))
+                                                                    uu___16)))
+                                                                    uu___15)))
+                                                                    uu___14)))
+                                                                    uu___14))
                                                                     | 
                                                                     Pulse_Syntax_Base.EffectAnnotSTT
                                                                     ->
@@ -2178,21 +2374,22 @@ let (check :
                                                                     (Obj.magic
                                                                     (FStar_Range.mk_range
                                                                     "Pulse.Checker.WithInv.fst"
-                                                                    (Prims.of_int (468))
+                                                                    (Prims.of_int (472))
                                                                     (Prims.of_int (14))
-                                                                    (Prims.of_int (468))
+                                                                    (Prims.of_int (472))
                                                                     (Prims.of_int (57)))))
                                                                     (FStar_Sealed.seal
                                                                     (Obj.magic
                                                                     (FStar_Range.mk_range
                                                                     "Pulse.Checker.WithInv.fst"
-                                                                    (Prims.of_int (469))
+                                                                    (Prims.of_int (473))
                                                                     (Prims.of_int (6))
-                                                                    (Prims.of_int (469))
+                                                                    (Prims.of_int (473))
                                                                     (Prims.of_int (59)))))
                                                                     (FStar_Tactics_Effect.lift_div_tac
                                                                     (fun
-                                                                    uu___9 ->
+                                                                    uu___13
+                                                                    ->
                                                                     Pulse_Typing.T_Lift
                                                                     (g, tm,
                                                                     c_out,
@@ -2204,7 +2401,8 @@ let (check :
                                                                     (g,
                                                                     c_out)))))
                                                                     (fun
-                                                                    uu___9 ->
+                                                                    uu___13
+                                                                    ->
                                                                     (fun d1
                                                                     ->
                                                                     Obj.magic
@@ -2218,30 +2416,33 @@ let (check :
                                                                     c_out)),
                                                                     d1))
                                                                     res_ppname))
-                                                                    uu___9)))
-                                                                    uu___9)))
-                                                                    uu___9)))
-                                                                    uu___9)))
-                                                                    uu___9)))
-                                                                    uu___8)))
-                                                                    uu___8)))
-                                                                    uu___8)))
-                                                                    uu___8)))
+                                                                    uu___13)))
+                                                                    uu___13)))
+                                                                    uu___13)))
+                                                                    uu___13)))
+                                                                    uu___13)))
+                                                                    uu___12)))
+                                                                    uu___12)))
+                                                                    uu___12)))
+                                                                    uu___12)))
+                                                                    uu___12)))
+                                                                    uu___11)))
+                                                                    uu___10)))
+                                                                    uu___10)))
                                                                     uu___8)))
                                                                     uu___7)))
+                                                                    uu___7)))
+                                                                    uu___7)))
+                                                                    uu___7)))
+                                                                    uu___7)))
+                                                                    uu___7)))
+                                                                    uu___7)))
+                                                                    uu___7)))
                                                                     uu___6)))
-                                                                    uu___6)))
-                                                                    uu___4)))
+                                                                    uu___5)))
+                                                                    uu___5)))
                                                                     uu___3)))
                                                                     uu___3)))
-                                                                    uu___3)))
-                                                                    uu___3)))
-                                                                    uu___3)))
-                                                                    uu___3)))
-                                                                    uu___3)))
-                                                                    uu___3)))
-                                                                    uu___2)))
-                                                                    uu___1)))
-                                                                    uu___1)))
-                                                            uu___1))) uu___1)))
-                                      uu___1))) uu___)
+                                                                uu___3)))
+                                                     uu___3))) uu___1)))
+                       uu___)
