pulse/lib/pulse/lib/Pulse.Lib.FlippableInv.fst
@@ -19,20 +19,35 @@ module Pulse.Lib.FlippableInv
 open Pulse.Lib.Pervasives
 module GR = Pulse.Lib.GhostReference
 
-let finv_p (p:vprop) (r : GR.ref bool) : vprop =
+let big_star (p q : vprop)
+: Lemma
+    (requires is_big p /\ is_big q)
+    (ensures is_big (p ** q))
+    [SMTPat (is_big (p ** q))] = big_star p q
+
+let big_exists (#a:Type u#a) (p: a -> vprop)
+: Lemma
+    (requires forall x. is_big (p x))
+    (ensures is_big (op_exists_Star p))
+    [SMTPat (is_big (op_exists_Star p))] = big_exists p
+
+let finv_p (p:vprop { is_big p }) (r : GR.ref bool) : v:vprop { is_big v } =
   exists* (b:bool). GR.pts_to r #one_half b ** (if b then p else emp)
 
 noeq
 type finv (p:vprop) = {
   r : GR.ref bool;
-  i : inv (finv_p p r);
+  i : iref;
+  p_big : squash (is_big p);
 }
 
-let off #p (fi : finv p) : vprop = GR.pts_to fi.r #one_half false
-let on  #p (fi : finv p) : vprop = GR.pts_to fi.r #one_half true
+let off #p (fi : finv p) : vprop =
+  GR.pts_to fi.r #one_half false ** inv fi.i (finv_p p fi.r)
+let on  #p (fi : finv p) : vprop =
+  GR.pts_to fi.r #one_half true ** inv fi.i (finv_p p fi.r)
 
 ```pulse
-fn __mk_finv (p:vprop)
+fn __mk_finv (p:vprop { is_big p })
    requires emp
    returns f:(finv p)
    ensures off f
@@ -43,41 +58,40 @@ fn __mk_finv (p:vprop)
         as (if false then p else emp);
    fold finv_p p r;
    let i = new_invariant (finv_p p r);
-   let fi = Mkfinv r i; // See #121
+   let fi = Mkfinv r i (() <: squash (is_big p)); // See #121
    rewrite (GR.pts_to r #one_half false)
         as (GR.pts_to fi.r #one_half false);
+   rewrite (inv i (finv_p p r))
+        as (inv fi.i (finv_p p fi.r));
    fold (off #p fi);
    fi
 }
 ```
 let mk_finv = __mk_finv
 
-let iname_of #p (f : finv p) : erased iname = name_of_inv f.i
+let iname_of #p (f : finv p) : erased iname = iname_of f.i
 
 ```pulse
 atomic
-fn _flip_on (#p:vprop) (fi : finv p)
+fn _flip_on (#p:vprop) (fi:finv p)
    requires off fi ** p
    ensures on fi
    opens add_iname emp_inames (iname_of fi)
 {
   open Pulse.Lib.GhostReference;
-  with_invariants fi.i {
-    unfold off fi;
-    unfold finv_p p fi.r;
-
+  unfold off;
+  with_invariants fi.i
+    returns _:unit
+    ensures inv fi.i (finv_p p fi.r) ** GR.pts_to fi.r #one_half true {
+    unfold finv_p;
     GR.gather2 fi.r;
-
-    rewrite (if false then p else emp)
-         as emp;
-
+    rewrite (if false then p else emp) as emp;
     fi.r := true;
-    
     GR.share2 fi.r;
-         
-    fold finv_p p fi.r;
-    fold (on fi)
-  }
+    rewrite p as (if true then p else emp);
+    fold (finv_p p fi.r);
+  };
+  fold (on fi)
 }
 ```
 let flip_on = _flip_on
@@ -90,22 +104,19 @@ fn _flip_off (#p:vprop) (fi : finv p)
    opens add_iname emp_inames (iname_of fi)
 {
   open Pulse.Lib.GhostReference;
-  with_invariants fi.i {
-    unfold on fi;
-    unfold finv_p p fi.r;
-
+  unfold on;
+  with_invariants fi.i
+    returns _:unit
+    ensures inv fi.i (finv_p p fi.r) ** GR.pts_to fi.r #one_half false ** p {
+    unfold finv_p;
     GR.gather2 fi.r;
-
+    rewrite (if true then p else emp) as p;
     fi.r := false;
-    
     GR.share2 fi.r;
-    
-    rewrite emp
-         as (if false then p else emp);
-         
-    fold finv_p p fi.r;
-    fold (off fi)
-  }
+    rewrite emp as (if false then p else emp);
+    fold (finv_p p fi.r);
+  };
+  fold (off fi)
 }
 ```
 let flip_off = _flip_off
